WBW-montgomery: Fill in most context variables

src/Arithmetic/MontgomeryReduction/WordByWord/Definition.v
@@ -1,81 +1,17 @@
 (*** Word-By-Word Montgomery Multiplication *)
 (** This file implements Montgomery Form, Montgomery Reduction, and
-    Montgomery Multiplication on an abstract [T].  We follow "Fast Prime
-    Field Elliptic Curve Cryptography with 256 Bit Primes",
-    https://eprint.iacr.org/2013/816.pdf. *)
-Require Import Coq.ZArith.ZArith.
-Require Import Crypto.Util.Notations.
-Require Import Crypto.Util.LetIn.
+    Montgomery Multiplication on an abstract [list ℤ].  We follow
+    "Fast Prime Field Elliptic Curve Cryptography with 256 Bit
+    Primes", https://eprint.iacr.org/2013/816.pdf. *)
+Require Import Coq.ZArith.BinInt.
+Require Import Crypto.Arithmetic.Saturated.
+Require Import Crypto.Arithmetic.MontgomeryReduction.WordByWord.Abstract.Definition.
 
-(** Quoting from page 7 of "Fast Prime
-    Field Elliptic Curve Cryptography with 256 Bit Primes",
-    https://eprint.iacr.org/2013/816.pdf: *)
-(** * Algorithm 1: Word-by-Word Montgomery Multiplication (WW-MM) *)
-(** Input: [p < 2ˡ] (odd modulus),
-           [0 ≤ a, b < p], [l = s×k]
-    Output: [a×b×2⁻ˡ mod p]
-    Pre-computed: [k0 = -p⁻¹ mod 2ˢ]
-    Flow
-<<
-1. T = a×b
- For i = 1 to k do
-   2. T1 = T mod 2ˢ
-   3. Y = T1 × k0 mod 2ˢ
-   4. T2 = Y × p
-   5. T3 = (T + T2)
-   6. T = T3 / 2ˢ
- End For
-7. If T ≥ p then X = T – p;
-      else X = T
-Return X
->> *)
-Local Open Scope Z_scope.
+Section redc.
+  (** XXX TODO: Figure out how to fill in these context variables *)
+  Context {mul_split : Z -> Z -> Z -> Z * Z} (* first argument is where to split output; [mul_split s x y] gives ((x * y) mod s, (x * y) / s) *).
 
-Section WordByWordMontgomery.
-  Local Coercion Z.pos : positive >-> Z.
-  Context
-    {T : Type}
-    {eval : T -> Z}
-    {numlimbs : T -> nat}
-    {zero : nat -> T}
-    {divmod : T -> T * Z} (* returns lowest limb and all-but-lowest-limb *)
-    {r : positive}
-    {scmul : Z -> T -> T} (* uses double-output multiply *)
-    {R : positive}
-    {add : T -> T -> T} (* joins carry *)
-    {drop_high : T -> T} (* drops the highest limb *)
-    (N : T).
-
-  (* Recurse for a as many iterations as A has limbs, varying A := A, S := 0, r, bounds *)
-  Section Iteration.
-    Context (B : T) (k : Z).
-    Context (A S : T).
-    (* Given A, B < R, we want to compute A * B / R mod N. R = bound 0 * ... * bound (n-1) *)
-    Local Definition A_a := dlet p := divmod A in p. Local Definition A' := fst A_a. Local Definition a := snd A_a.
-    Local Definition S1 := add S (scmul a B).
-    Local Definition s := snd (divmod S1).
-    Local Definition q := s * k mod r.
-    Local Definition S2 := add S1 (scmul q N).
-    Local Definition S3 := fst (divmod S2).
-    Local Definition S4 := drop_high S3.
-  End Iteration.
-
-  Section loop.
-    Context (A B : T) (k : Z) (S' : T).
-
-    Definition redc_body : T * T -> T * T
-      := fun '(A, S') => (A' A, S4 B k A S').
-
-    Fixpoint redc_loop (count : nat) : T * T -> T * T
-      := match count with
-         | O => fun A_S => A_S
-         | S count' => fun A_S => redc_loop count' (redc_body A_S)
-         end.
-
-    Definition redc : T
-      := snd (redc_loop (numlimbs A) (A, zero (1 + numlimbs B))).
-  End loop.
-End WordByWordMontgomery.
-
-Create HintDb word_by_word_montgomery.
-Hint Unfold S4 S3 S2 q s S1 a A' A_a Let_In : word_by_word_montgomery.
+  (** XXX TODO: pick better names for the arguments to this definition. *)
+  Definition redc {r : positive} {R_numlimbs : nat} (N A B : T) (k : Z) : T
+    := @redc T numlimbs zero divmod r (@scmul (Z.pos r) mul_split) (@add (Z.pos r)) (@drop_high (S R_numlimbs)) N A B k.
+End redc.
