src/Arithmetic/MontgomeryReduction/WordByWord/Abstract/Proofs.v
@@ -1,0 +1,486 @@
+(*** Word-By-Word Montgomery Multiplication Proofs *)
+Require Import Coq.Arith.Arith.
+Require Import Coq.ZArith.BinInt Coq.ZArith.ZArith Coq.ZArith.Zdiv Coq.micromega.Lia.
+Require Import Crypto.Util.LetIn.
+Require Import Crypto.Util.Prod.
+Require Import Crypto.Util.NatUtil.
+Require Import Crypto.Util.ZUtil.
+Require Import Crypto.Arithmetic.ModularArithmeticTheorems Crypto.Spec.ModularArithmetic.
+Require Import Crypto.Arithmetic.MontgomeryReduction.WordByWord.Abstract.Definition.
+Require Import Crypto.Algebra.Ring.
+Require Import Crypto.Util.Sigma.
+Require Import Crypto.Util.Tactics.SetEvars.
+Require Import Crypto.Util.Tactics.SubstEvars.
+Require Import Crypto.Util.Tactics.DestructHead.
+Local Open Scope Z_scope.
+
+Section WordByWordMontgomery.
+  Context
+    {T : Type}
+    {eval : T -> Z}
+    {numlimbs : T -> nat}
+    {zero : nat -> T}
+    {divmod : T -> T * Z} (* returns lowest limb and all-but-lowest-limb *)
+    {r : positive}
+    {r_big : r > 1}
+    {small : T -> Prop}
+    {eval_zero : forall n, eval (zero n) = 0}
+    {numlimbs_zero : forall n, numlimbs (zero n) = n}
+    {eval_div : forall v, small v -> eval (fst (divmod v)) = eval v / r}
+    {eval_mod : forall v, small v -> snd (divmod v) = eval v mod r}
+    {small_div : forall v, small v -> small (fst (divmod v))}
+    {numlimbs_div : forall v, numlimbs (fst (divmod v)) = pred (numlimbs v)}
+    {scmul : Z -> T -> T} (* uses double-output multiply *)
+    {eval_scmul: forall a v, eval (scmul a v) = a * eval v}
+    {numlimbs_scmul : forall a v, 0 <= a < r -> numlimbs (scmul a v) = S (numlimbs v)}
+    {R : positive}
+    {R_numlimbs : nat}
+    {R_correct : R = r^Z.of_nat R_numlimbs :> Z}
+    {add : T -> T -> T} (* joins carry *)
+    {eval_add : forall a b, eval (add a b) = eval a + eval b}
+    {small_add : forall a b, small (add a b)}
+    {numlimbs_add : forall a b, numlimbs (add a b) = Datatypes.S (max (numlimbs a) (numlimbs b))}
+    {drop_high : T -> T} (* drops things after [S R_numlimbs] *)
+    {eval_drop_high : forall v, small v -> eval (drop_high v) = eval v mod (r * r^Z.of_nat R_numlimbs)}
+    {numlimbs_drop_high : forall v, numlimbs (drop_high v) = min (numlimbs v) (S R_numlimbs)}
+    (N : T) (Npos : positive) (Npos_correct: eval N = Z.pos Npos)
+    (N_lt_R : eval N < R)
+    (B : T)
+    (B_bounds : 0 <= eval B < R)
+    ri (ri_correct : r*ri mod (eval N) = 1 mod (eval N)).
+  Context (k : Z) (k_correct : k * eval N mod r = -1).
+
+  Create HintDb push_numlimbs discriminated.
+  Create HintDb push_eval discriminated.
+  Local Ltac t_small :=
+    repeat first [ assumption
+                 | apply small_add
+                 | apply small_div
+                 | apply Z_mod_lt
+                 | solve [ auto ]
+                 | lia
+                 | progress autorewrite with push_eval
+                 | progress autorewrite with push_numlimbs ].
+  Hint Rewrite
+       eval_zero
+       eval_div
+       eval_mod
+       eval_add
+       eval_scmul
+       eval_drop_high
+       using (repeat autounfold with word_by_word_montgomery; t_small)
+    : push_eval.
+  Hint Rewrite
+       numlimbs_zero
+       numlimbs_div
+       numlimbs_add
+       numlimbs_scmul
+       numlimbs_drop_high
+       using (repeat autounfold with word_by_word_montgomery; t_small)
+    : push_numlimbs.
+  Hint Rewrite <- Max.succ_max_distr pred_Sn Min.succ_min_distr : push_numlimbs.
+
+
+  (* Recurse for a as many iterations as A has limbs, varying A := A, S := 0, r, bounds *)
+  Section Iteration.
+    Context (A S : T)
+            (small_A : small A)
+            (S_nonneg : 0 <= eval S).
+    (* Given A, B < R, we want to compute A * B / R mod N. R = bound 0 * ... * bound (n-1) *)
+
+    Local Coercion eval : T >-> Z.
+
+    Local Notation a := (@WordByWord.Abstract.Definition.a T divmod A).
+    Local Notation A' := (@WordByWord.Abstract.Definition.A' T divmod A).
+    Local Notation S1 := (@WordByWord.Abstract.Definition.S1 T divmod scmul add B A S).
+    Local Notation S2 := (@WordByWord.Abstract.Definition.S2 T divmod r scmul add N B k A S).
+    Local Notation S3 := (@WordByWord.Abstract.Definition.S3 T divmod r scmul add N B k A S).
+    Local Notation S4 := (@WordByWord.Abstract.Definition.S4 T divmod r scmul add drop_high N B k A S).
+
+    Lemma S3_bound
+      : eval S < eval N + eval B
+        -> eval S3 < eval N + eval B.
+    Proof.
+      assert (Hmod : forall a b, 0 < b -> a mod b <= b - 1)
+        by (intros x y; pose proof (Z_mod_lt x y); omega).
+      intro HS.
+      unfold S3, WordByWord.Abstract.Definition.S2, WordByWord.Abstract.Definition.S1.
+      autorewrite with push_eval; [].
+      eapply Z.le_lt_trans.
+      { transitivity ((N+B-1 + (r-1)*B + (r-1)*N) / r);
+          [ | set_evars; ring_simplify_subterms; subst_evars; reflexivity ].
+        Z.peel_le; repeat apply Z.add_le_mono; repeat apply Z.mul_le_mono_nonneg; try lia;
+          repeat autounfold with word_by_word_montgomery;
+          autorewrite with push_eval;
+            try Z.zero_bounds;
+            auto with lia. }
+      rewrite (Z.mul_comm _ r), <- Z.add_sub_assoc, <- Z.add_opp_r, !Z.div_add_l' by lia.
+      autorewrite with zsimplify.
+      omega.
+    Qed.
+
+    Lemma small_A'
+      : small A'.
+    Proof.
+      repeat autounfold with word_by_word_montgomery; auto.
+    Qed.
+
+    Lemma small_S3
+      : small S3.
+    Proof. repeat autounfold with word_by_word_montgomery; t_small. Qed.
+
+    Lemma S3_nonneg : 0 <= eval S3.
+    Proof.
+      repeat autounfold with word_by_word_montgomery;
+        autorewrite with push_eval; [].
+      rewrite ?Npos_correct; Z.zero_bounds; lia.
+    Qed.
+
+    Lemma S4_nonneg : 0 <= eval S4.
+    Proof. unfold S4; rewrite eval_drop_high by apply small_S3; Z.zero_bounds. Qed.
+
+    Lemma S4_bound
+      : eval S < eval N + eval B
+        -> eval S4 < eval N + eval B.
+    Proof.
+      intro H; pose proof (S3_bound H); pose proof S3_nonneg.
+      unfold S4.
+      rewrite eval_drop_high by apply small_S3.
+      rewrite Z.mod_small by nia.
+      assumption.
+    Qed.
+
+    Lemma numlimbs_S4 : numlimbs S4 = min (max (1 + numlimbs S) (1 + max (1 + numlimbs B) (numlimbs N))) (1 + R_numlimbs).
+    Proof.
+      cbn [plus].
+      repeat autounfold with word_by_word_montgomery.
+      repeat autorewrite with push_numlimbs.
+      change Init.Nat.max with Nat.max.
+      rewrite <- ?(Max.max_assoc (numlimbs S)).
+      reflexivity.
+    Qed.
+
+    Lemma S1_eq : eval S1 = S + a*B.
+    Proof.
+      cbv [S1 a WordByWord.Abstract.Definition.A'].
+      repeat autorewrite with push_eval.
+      reflexivity.
+    Qed.
+
+    Lemma S2_mod_N : (eval S2) mod N = (S + a*B) mod N.
+    Proof.
+      cbv [S2 WordByWord.Abstract.Definition.q WordByWord.Abstract.Definition.s]; autorewrite with push_eval zsimplify. rewrite S1_eq. reflexivity.
+    Qed.
+
+    Lemma S2_mod_r : S2 mod r = 0.
+      cbv [S2 WordByWord.Abstract.Definition.q WordByWord.Abstract.Definition.s]; autorewrite with push_eval.
+      assert (r > 0) by lia.
+      assert (Hr : (-(1 mod r)) mod r = r - 1 /\ (-(1)) mod r = r - 1).
+      { destruct (Z.eq_dec r 1) as [H'|H'].
+        { rewrite H'; split; reflexivity. }
+        { rewrite !Z_mod_nz_opp_full; rewrite ?Z.mod_mod; Z.rewrite_mod_small; [ split; reflexivity | omega.. ]. } }
+      autorewrite with pull_Zmod.
+      replace 0 with (0 mod r) by apply Zmod_0_l.
+      eapply F.eq_of_Z_iff.
+      repeat rewrite ?F.of_Z_add, ?F.of_Z_mul, <-?F.of_Z_mod.
+      rewrite <-Algebra.Hierarchy.associative.
+      replace ((F.of_Z r k * F.of_Z r (eval N))%F) with (F.opp (m:=r) F.one).
+      { cbv [F.of_Z F.add]; simpl.
+        apply path_sig_hprop; [ intro; exact HProp.allpath_hprop | ].
+        simpl.
+        rewrite (proj1 Hr), Z.mul_sub_distr_l.
+        push_Zmod; pull_Zmod.
+        autorewrite with zsimplify; reflexivity. }
+      { rewrite <- F.of_Z_mul.
+        rewrite F.of_Z_mod.
+        rewrite k_correct.
+        cbv [F.of_Z F.add F.opp F.one]; simpl.
+        change (-(1)) with (-1) in *.
+        apply path_sig_hprop; [ intro; exact HProp.allpath_hprop | ]; simpl.
+        rewrite (proj1 Hr), (proj2 Hr); reflexivity. }
+    Qed.
+
+    Lemma S3_mod_N
+      : S3 mod N = (S + a*B)*ri mod N.
+    Proof.
+      cbv [S3]; autorewrite with push_eval cancel_pair.
+      pose proof fun a => Z.div_to_inv_modulo N a r ri eq_refl ri_correct as HH;
+                            cbv [Z.equiv_modulo] in HH; rewrite HH; clear HH.
+      etransitivity; [rewrite (fun a => Z.mul_mod_l a ri N)|
+                      rewrite (fun a => Z.mul_mod_l a ri N); reflexivity].
+      rewrite <-S2_mod_N; repeat (f_equal; []); autorewrite with push_eval.
+      autorewrite with push_Zmod;
+        rewrite S2_mod_r;
+        autorewrite with zsimplify.
+      reflexivity.
+    Qed.
+
+    Lemma S4_mod_N
+          (Hbound : eval S < eval N + eval B)
+      : S4 mod N = (S + a*B)*ri mod N.
+    Proof.
+      pose proof (S3_bound Hbound); pose proof S3_nonneg.
+      unfold S4; autorewrite with push_eval.
+      rewrite (Z.mod_small _ (r * _)) by nia.
+      apply S3_mod_N.
+    Qed.
+  End Iteration.
+
+  Local Notation redc_body := (@redc_body T divmod r scmul add drop_high N B k).
+  Local Notation redc_loop := (@redc_loop T divmod r scmul add drop_high N B k).
+  Local Notation redc A := (@redc T numlimbs zero divmod r scmul add drop_high N A B k).
+
+  Lemma redc_loop_comm_body count
+    : forall A_S, redc_loop count (redc_body A_S) = redc_body (redc_loop count A_S).
+  Proof.
+    induction count as [|count IHcount]; try reflexivity.
+    simpl; intro; rewrite IHcount; reflexivity.
+  Qed.
+
+  Section body.
+    Context (A_S : T * T).
+    Let A:=fst A_S.
+    Let S:=snd A_S.
+    Let A_a:=divmod A.
+    Let a:=snd A_a.
+    Context (small_A : small A)
+            (S_bound : 0 <= eval S < eval N + eval B).
+
+    Lemma small_fst_redc_body : small (fst (redc_body A_S)).
+    Proof. destruct A_S; apply small_A'; assumption. Qed.
+    Lemma snd_redc_body_nonneg : 0 <= eval (snd (redc_body A_S)).
+    Proof. destruct A_S; apply S4_nonneg; assumption. Qed.
+
+    Lemma snd_redc_body_mod_N
+      : (eval (snd (redc_body A_S))) mod (eval N) = (eval S + a*eval B)*ri mod (eval N).
+    Proof. destruct A_S; apply S4_mod_N; auto; omega. Qed.
+
+    Lemma fst_redc_body
+      : (eval (fst (redc_body A_S))) = eval (fst A_S) / r.
+    Proof.
+      destruct A_S; simpl; unfold WordByWord.Abstract.Definition.A', WordByWord.Abstract.Definition.A_a, Let_In, a, A_a, A; simpl.
+      autorewrite with push_eval.
+      reflexivity.
+    Qed.
+
+    Lemma fst_redc_body_mod_N
+      : (eval (fst (redc_body A_S))) mod (eval N) = ((eval (fst A_S) - a)*ri) mod (eval N).
+    Proof.
+      rewrite fst_redc_body.
+      etransitivity; [ eapply Z.div_to_inv_modulo; try eassumption; lia | ].
+      unfold a, A_a, A.
+      autorewrite with push_eval.
+      reflexivity.
+    Qed.
+
+    Lemma redc_body_bound
+      : eval S < eval N + eval B
+        -> eval (snd (redc_body A_S)) < eval N + eval B.
+    Proof.
+      destruct A_S; apply S4_bound; unfold S in *; cbn [snd] in *; try assumption; try omega.
+    Qed.
+
+    Lemma numlimbs_redc_body : numlimbs (snd (redc_body A_S))
+                               = min (max (1 + numlimbs (snd A_S)) (1 + max (1 + numlimbs B) (numlimbs N))) (1 + R_numlimbs).
+    Proof. destruct A_S; apply numlimbs_S4; assumption. Qed.
+  End body.
+
+  Local Arguments Z.pow !_ !_.
+  Local Arguments Z.of_nat !_.
+  Local Ltac induction_loop count IHcount
+    := induction count as [|count IHcount]; intros; cbn [redc_loop] in *; [ | rewrite redc_loop_comm_body in * ].
+  Lemma redc_loop_good A_S count
+        (Hsmall : small (fst A_S))
+        (Hbound : 0 <= eval (snd A_S) < eval N + eval B)
+    : small (fst (redc_loop count A_S))
+      /\ 0 <= eval (snd (redc_loop count A_S)) < eval N + eval B.
+  Proof.
+    induction_loop count IHcount; auto; [].
+    change (id (0 <= eval B < R)) in B_bounds (* don't let [destruct_head'_and] loop *).
+    destruct_head'_and.
+    repeat first [ apply conj
+                 | apply small_fst_redc_body
+                 | apply redc_body_bound
+                 | apply snd_redc_body_nonneg
+                 | solve [ auto ] ].
+  Qed.
+
+  Lemma redc_loop_bound A_S count
+        (Hsmall : small (fst A_S))
+        (Hbound : 0 <= eval (snd A_S) < eval N + eval B)
+    : 0 <= eval (snd (redc_loop count A_S)) < eval N + eval B.
+  Proof. apply redc_loop_good; assumption. Qed.
+
+  Local Ltac t_min_max_step _ :=
+    match goal with
+    | [ |- context[Init.Nat.max ?x ?y] ]
+      => first [ rewrite (Max.max_l x y) by omega
+               | rewrite (Max.max_r x y) by omega ]
+    | [ |- context[Init.Nat.min ?x ?y] ]
+      => first [ rewrite (Min.min_l x y) by omega
+               | rewrite (Min.min_r x y) by omega ]
+    | _ => progress change Init.Nat.max with Nat.max
+    | _ => progress change Init.Nat.min with Nat.min
+    end.
+
+  Lemma numlimbs_redc_loop A_S count
+        (Hsmall : small (fst A_S))
+        (Hbound : 0 <= eval (snd A_S) < eval N + eval B)
+        (Hnumlimbs : (R_numlimbs <= numlimbs (snd A_S))%nat)
+    : numlimbs (snd (redc_loop count A_S))
+      = match count with
+        | O => numlimbs (snd A_S)
+        | S _ => 1 + R_numlimbs
+        end%nat.
+  Proof.
+    assert (Hgen
+            : numlimbs (snd (redc_loop count A_S))
+              = match count with
+                | O => numlimbs (snd A_S)
+                | S _ => min (max (count + numlimbs (snd A_S)) (1 + max (1 + numlimbs B) (numlimbs N))) (1 + R_numlimbs)
+                end).
+    { induction_loop count IHcount; [ reflexivity | ].
+      rewrite numlimbs_redc_body by (try apply redc_loop_good; auto).
+      rewrite IHcount; clear IHcount.
+      destruct count; [ reflexivity | ].
+      destruct (Compare_dec.le_lt_dec (1 + max (1 + numlimbs B) (numlimbs N)) (S count + numlimbs (snd A_S))),
+      (Compare_dec.le_lt_dec (1 + R_numlimbs) (S count + numlimbs (snd A_S))),
+      (Compare_dec.le_lt_dec (1 + R_numlimbs) (1 + max (1 + numlimbs B) (numlimbs N)));
+        repeat first [ reflexivity
+                     | t_min_max_step ()
+                     | progress autorewrite with push_numlimbs
+                     | rewrite Nat.min_comm, Nat.min_max_distr ]. }
+    rewrite Hgen; clear Hgen.
+    destruct count; [ reflexivity | ].
+    repeat apply Max.max_case_strong; apply Min.min_case_strong; omega.
+  Qed.
+
+
+  Lemma fst_redc_loop A_S count
+        (Hsmall : small (fst A_S))
+        (Hbound : 0 <= eval (snd A_S) < eval N + eval B)
+    : eval (fst (redc_loop count A_S)) = eval (fst A_S) / r^(Z.of_nat count).
+  Proof.
+    induction_loop count IHcount.
+    { simpl; autorewrite with zsimplify; reflexivity. }
+    { rewrite fst_redc_body, IHcount
+        by (apply redc_loop_good; auto).
+      rewrite Zdiv_Zdiv by Z.zero_bounds.
+      rewrite <- (Z.pow_1_r r) at 2.
+      rewrite <- Z.pow_add_r by lia.
+      replace (Z.of_nat count + 1) with (Z.of_nat (S count)) by (simpl; lia).
+      reflexivity. }
+  Qed.
+
+  Lemma fst_redc_loop_mod_N A_S count
+        (Hsmall : small (fst A_S))
+        (Hbound : 0 <= eval (snd A_S) < eval N + eval B)
+    : eval (fst (redc_loop count A_S)) mod (eval N)
+      = (eval (fst A_S) - eval (fst A_S) mod r^Z.of_nat count)
+        * ri^(Z.of_nat count) mod (eval N).
+  Proof.
+    rewrite fst_redc_loop by assumption.
+    destruct count.
+    { simpl; autorewrite with zsimplify; reflexivity. }
+    { etransitivity;
+        [ eapply Z.div_to_inv_modulo;
+          try solve [ eassumption
+                    | apply Z.lt_gt, Z.pow_pos_nonneg; lia ]
+        | ].
+      { erewrite <- Z.pow_mul_l, <- Z.pow_1_l.
+        { apply Z.pow_mod_Proper; [ eassumption | reflexivity ]. }
+        { lia. } }
+      reflexivity. }
+  Qed.
+
+  Local Arguments Z.pow : simpl never.
+  Lemma snd_redc_loop_mod_N A_S count
+        (Hsmall : small (fst A_S))
+        (Hbound : 0 <= eval (snd A_S) < eval N + eval B)
+    : (eval (snd (redc_loop count A_S))) mod (eval N)
+      = ((eval (snd A_S) + (eval (fst A_S) mod r^(Z.of_nat count))*eval B)*ri^(Z.of_nat count)) mod (eval N).
+  Proof.
+    induction_loop count IHcount.
+    { simpl; autorewrite with zsimplify; reflexivity. }
+    { simpl; rewrite snd_redc_body_mod_N
+        by (apply redc_loop_good; auto).
+      push_Zmod; rewrite IHcount; pull_Zmod.
+      autorewrite with push_eval; [ | apply redc_loop_good; auto.. ]; [].
+      match goal with
+      | [ |- ?x mod ?N = ?y mod ?N ]
+        => change (Z.equiv_modulo N x y)
+      end.
+      destruct A_S as [A S].
+      cbn [fst snd].
+      change (Z.pos (Pos.of_succ_nat ?n)) with (Z.of_nat (Datatypes.S n)).
+      rewrite !Z.mul_add_distr_r.
+      rewrite <- !Z.mul_assoc.
+      replace (ri^(Z.of_nat count) * ri) with (ri^(Z.of_nat (Datatypes.S count)))
+        by (change (Datatypes.S count) with (1 + count)%nat;
+            autorewrite with push_Zof_nat; rewrite Z.pow_add_r by lia; simpl Z.succ; rewrite Z.pow_1_r; nia).
+      rewrite <- !Z.add_assoc.
+      apply Z.add_mod_Proper; [ reflexivity | ].
+      unfold Z.equiv_modulo; push_Zmod; rewrite (Z.mul_mod_l (_ mod r) _ (eval N)).
+      rewrite fst_redc_loop by (try apply redc_loop_good; auto; omega).
+      cbn [fst].
+      rewrite Z.mod_pull_div by lia.
+      erewrite Z.div_to_inv_modulo;
+        [
+        | solve [ eassumption | apply Z.lt_gt, Z.pow_pos_nonneg; lia ]
+        | erewrite <- Z.pow_mul_l, <- Z.pow_1_l;
+          [ apply Z.pow_mod_Proper; [ eassumption | reflexivity ]
+          | lia ] ].
+      pull_Zmod.
+      match goal with
+      | [ |- ?x mod ?N = ?y mod ?N ]
+        => change (Z.equiv_modulo N x y)
+      end.
+      repeat first [ rewrite <- !Z.pow_succ_r, <- !Nat2Z.inj_succ by lia
+                   | rewrite (Z.mul_comm _ ri)
+                   | rewrite (Z.mul_assoc _ ri _)
+                   | rewrite (Z.mul_comm _ (ri^_))
+                   | rewrite (Z.mul_assoc _ (ri^_) _) ].
+      repeat first [ rewrite <- Z.mul_assoc
+                   | rewrite <- Z.mul_add_distr_l
+                   | rewrite (Z.mul_comm _ (eval B))
+                   | rewrite !Nat2Z.inj_succ, !Z.pow_succ_r by lia;
+                     rewrite <- Znumtheory.Zmod_div_mod by (apply Z.divide_factor_r || Z.zero_bounds)
+                   | rewrite Zplus_minus
+                   | reflexivity ]. }
+  Qed.
+
+  Lemma redc_bound A
+        (small_A : small A)
+    : 0 <= eval (redc A) < eval N + eval B.
+  Proof.
+    unfold redc.
+    apply redc_loop_good; simpl; autorewrite with push_eval;
+      rewrite ?Npos_correct; auto; lia.
+  Qed.
+
+  Lemma numlimbs_redc_gen A (small_A : small A) (Hnumlimbs : (R_numlimbs <= numlimbs B)%nat)
+    : numlimbs (redc A)
+      = match numlimbs A with
+        | O => S (numlimbs B)
+        | _ => S R_numlimbs
+        end.
+  Proof.
+    unfold redc; rewrite numlimbs_redc_loop by (cbn [fst snd]; t_small);
+      cbn [snd]; rewrite ?numlimbs_zero.
+    reflexivity.
+  Qed.
+  Lemma numlimbs_redc A (small_A : small A) (Hnumlimbs : R_numlimbs = numlimbs B)
+    : numlimbs (redc A) = S (numlimbs B).
+  Proof. rewrite numlimbs_redc_gen; subst; auto; destruct (numlimbs A); reflexivity. Qed.
+
+  Lemma redc_mod_N A (small_A : small A) (A_bound : 0 <= eval A < r ^ Z.of_nat (numlimbs A))
+    : (eval (redc A)) mod (eval N) = (eval A * eval B * ri^(Z.of_nat (numlimbs A))) mod (eval N).
+  Proof.
+    unfold redc.
+    rewrite snd_redc_loop_mod_N; cbn [fst snd];
+      autorewrite with push_eval zsimplify;
+      [ | rewrite ?Npos_correct; auto; lia.. ].
+    Z.rewrite_mod_small.
+    reflexivity.
+  Qed.
+End WordByWordMontgomery.
